src/program_proof/mvcc/tuple_mk.v
@@ -75,7 +75,18 @@ Proof.
   (***********************************************************)
   (* return tuple                                            *)
   (***********************************************************)
-  iMod (min_tid_lb_zero γ) as "#Hlb".
+  
+  (* Obtain [min_tid_lb γ 0]. *)
+  iInv "Hinvgc" as "> HinvgcO" "HinvgcC".
+  iDestruct (min_tid_lb_zero γ (1 / 2) with "[HinvgcO]") as "#Hlb".
+  { unfold mvcc_inv_gc_def.
+    iApply (big_sepL_mono with "HinvgcO").
+    iIntros (sidN sid) "%Hlookup H".
+    iDestruct "H" as (tids tidmin) "(_ & H & _)".
+    by eauto.
+  }
+  iMod ("HinvgcC" with "HinvgcO") as "_".
+  
   set P := (own_tuple tuple key γ)%I.
   iMod (alloc_lock mvccN _ latch P with "[$Hfree] [-latch rcond HΦ]") as "#Hlock".
   { iNext.
